coq/variant/rules_inf2.v
@@ -1,4 +1,4 @@
-(* !!! WARNING: AUTO GENERATED. DO NOT MODIFY !!! *)
+Require Import Coq.Arith.Wf_nat.
 Require Import Coq.Logic.FunctionalExtensionality.
 Require Import Coq.Program.Equality.
 
