spec/embeded_def.v
@@ -1,0 +1,5 @@
+Definition disjointSpec A B :=
+  forall C, sub A C -> sub B C -> topLike C.
+
+Definition consistencySpec v1 v2 :=
+  forall A v1' v2', TypedReduce v1 A v1' -> TypedReduce v2 A v2' -> v1' = v2'.
